\p
\begin{enumerate}
\item
$$\frac{x - 3}{x^2 - 3x + 2} = \frac{2}{x - 1} - \frac{1}{x - 2} = -\frac{2}{1 - x} + \frac{\frac{1}{2}}{1 - \frac{x}{2}}$$
ضریب
$x^{50}$
برابر است با:
$$-2 + \frac{1}{2}(\frac{1}{2^{50}})$$
\item
$$a_n - a_{n-1} = a_{n-1} + a_{n-2} + \cdots + a_0$$
اگر به جای
$n$
،
$n - 1$
قرار دهیم:
$$a_{n-1} - a_{n-2} = a_{n-2} + a_{n-3} + \cdots + a_0$$
با کم کردن دو معادله‌ی بالا از هم داریم:
$$a_n - 2a_{n-1} + a_{n-2} = a_{n-1}$$
$$a_n = 3a_{n-1} - a_{n-2} \Rightarrow x^2 - 3x + 1 = 0 \Rightarrow \frac{3 \pm \sqrt{5}}{2}$$
$$a_n = r(\frac{3 + \sqrt{5}}{2})^n + s(\frac{3 - \sqrt{5}}{2})^n$$
معادله بالا را با
$a_0$
و
$a_1$
حل می‌کنیم.
\end{enumerate}
