\p
\begin{enumerate}
\item
برای حل این قسمت از سوال از بسط دوجمله‌ای استفاده می‌کنیم:
$$(x^2 + x^3 + x^4 + x^5 + x^6 + x^7)^4 = x^8(1 + x + x^2 + x^3 + x^4 + x^5)^4 =$$
$$ x^8(1 - x^6)^4(1 - x)^{-4} = x^8(1 + \binom 4 1 (-x^6) + \binom 4 2 (-x^6)^2 + \cdots)\times$$
$$(1 + \binom{1+3}{1}x + \binom{2 + 3}{2}x^2 + \cdots + \binom{r + 3}{r}x^r + \cdots)$$
توان
$x^8$
برابر است با:
$$\binom{13}{10} - \binom{4}{1}\binom{7}{4}$$
\item
از ضریب دوجمله‌ای استفاده می‌کنیم:
$$(1-4x)^5 = 1 + \binom{1+4}{1}(4x) + \binom{2+4}{2}(4x)^2 + \binom{r+4}{4}(4x)^r + \cdots$$
توان
$x^{12}$
برابر است با:
$$\binom{12+4}{12}4^{12} = \binom{16}{12}4^{12}$$
\end{enumerate}