\p
\begin{enumerate}
\item
از توابع مولد استفاده می کنیم:
$$(x^2 + x^3 + x^4 + \cdots)^3 = \frac{x^6}{(1-3)^3} = x^6(1-3)^{-3}$$
ضریب
$x^{10}$
در عبارت بالا برابر است با:
$$\binom{4+3-1}{4} = \binom{6}{4}$$
\item
$$(1 + x + x^2 + \cdots)^2(1 + x + x^2) = (1-x)^{-2}(1 + x + x^2) = $$
$$(1 - x)^{-2} \frac{1-x^3}{1-x} = (1-x)^{-3}(1-x^3)$$
ضریب
$x^{10}$
در عبارت بالا برابر است با:
$$\binom{12}{10} - \binom{9}{7}$$
\item
$$(1 + x + x^2 + \cdots)^2(1 + x^2 + x^4 + \cdots) = (1 - x)^{-2}(1 + x^2 + x^4 + x^6 + x^8 + x^{10} + \cdots)$$
$$\Rightarrow \sum_{k=0}^{5}\binom{11 - 2k}{10 - 2k}$$
\end{enumerate}
